@prefix rdf:     <http://www.w3.org/1999/02/22-rdf-syntax-ns#> .
@prefix rdfs:    <http://www.w3.org/2000/01/rdf-schema#> .
@prefix owl:     <http://www.w3.org/2002/07/owl#> .
@prefix qb: 	 <http://purl.org/linked-data/cube#> .
@prefix ler: 	 <http://bit.ly/linked-edit-rules#> .

ler:EditRule a rdfs:Class, owl:Class;
    rdfs:label "Linked Edit Rule"@en;
    rdfs:comment "An edit rule defines a statistical constraint over RDF Data Cubes on certain components and a scope"@en;
    rdfs:seeAlso <https://github.com/albertmeronyo/ConceptDrift/tree/master/rules>
.

ler:scope a rdf:Property ;
    rdfs:range qb:ObservationGroup ;
    rdfs:domain ler:EditRule ;
    rdfs:label "LER Scope"@en ;
    rdfs:comment "The scope of an edit rule indicates whether it constraints observations, slices or datasets"@en
.

ler:component a rdf:Property ;
    rdfs:range qb:ComponentProperty ;
    rdfs:domain ler:EditRule ;
    rdfs:label "LER Component"@en ;
    rdfs:comment "The component of an edit rule indicates the dimension, attribute or measure it constraints"@en
.

ler:inconsistentWith a rdf:Property ;
    rdfs:range rdfs:Resource ; # Ideally bodies of oa:Annotation
    rdfs:domain ler:EditRule ;
    rdfs:label "LER Inconsistent With"@en ;
    rdfs:comment "Indicates that the annotated target is inconsistent with the Linked Edit Rule of the predicate"@en
.